core/TotalMapSimulations.v
@@ -37,7 +37,7 @@ Class MultiParamsNameTotalMapBijective `(M : MultiParamsNameTotalMap) :=
     tot_map_name_inverse_inv : forall n, tot_map_name (tot_map_name_inv n) = n ;
   }.
 
-Class MultiParamsTotalMap
+Class MultiParamsMsgTotalMap
  (B0 : BaseParams) (B1 : BaseParams)
  (P0 : MultiParams B0) (P1 : MultiParams B1) :=
   {
@@ -52,7 +52,7 @@ Context {multi_fst : MultiParams base_fst}.
 Context {multi_snd : MultiParams base_snd}.
 Context {base_map : BaseParamsTotalMap base_fst base_snd}.
 Context {name_map : MultiParamsNameTotalMap multi_fst multi_snd}.
-Context {multi_map : MultiParamsTotalMap multi_fst multi_snd}.
+Context {msg_map : MultiParamsMsgTotalMap multi_fst multi_snd}.
 
 Definition tot_map_name_msgs :=
   map (fun nm => (tot_map_name (fst nm), tot_map_msg (snd nm))).
@@ -72,14 +72,18 @@ Class MultiParamsTotalMapCongruency
   (P0 : MultiParams B0) (P1 : MultiParams B1)
   (B : BaseParamsTotalMap B0 B1) 
   (N : MultiParamsNameTotalMap P0 P1)
-  (P : MultiParamsTotalMap P0 P1) :=
+  (P : MultiParamsMsgTotalMap P0 P1) :=
   {
-    tot_init_handlers_eq : forall n, tot_map_data (init_handlers n) = init_handlers (tot_map_name n) ;
-    tot_net_handlers_eq : forall me src m st, tot_mapped_net_handlers me src m st = 
+    tot_init_handlers_eq : forall n, 
+      tot_map_data (init_handlers n) = init_handlers (tot_map_name n) ;
+    tot_net_handlers_eq : forall me src m st, 
+      tot_mapped_net_handlers me src m st = 
       net_handlers (tot_map_name me) (tot_map_name src) (tot_map_msg m) (tot_map_data st) ;
-    tot_input_handlers_eq : forall me inp st, tot_mapped_input_handlers me inp st = 
+    tot_input_handlers_eq : forall me inp st, 
+      tot_mapped_input_handlers me inp st = 
       input_handlers (tot_map_name me) (tot_map_input inp) (tot_map_data st) ;
-    tot_map_output_injective : forall o o', tot_map_output o = tot_map_output o' -> o = o'
+    tot_map_output_injective : forall o o', 
+      tot_map_output o = tot_map_output o' -> o = o'
   }.
 
 Class FailureParamsTotalMapCongruency 
@@ -97,14 +101,15 @@ Class NameOverlayParamsTotalMapCongruency
   (O0 : NameOverlayParams P0) (O1 : NameOverlayParams P1)
   (N : MultiParamsNameTotalMap P0 P1) :=
   {
-    tot_adjacent_to_fst_snd : forall n n', adjacent_to n n' <-> adjacent_to (tot_map_name n) (tot_map_name n')
+    tot_adjacent_to_fst_snd : forall n n', 
+      adjacent_to n n' <-> adjacent_to (tot_map_name n) (tot_map_name n')
   }.
 
 Class FailMsgParamsTotalMapCongruency 
   (B0 : BaseParams) (B1 : BaseParams)
   (P0 : MultiParams B0) (P1 : MultiParams B1)
   (F0 : FailMsgParams P0) (F1 : FailMsgParams P1)
-  (P : MultiParamsTotalMap P0 P1) :=
+  (P : MultiParamsMsgTotalMap P0 P1) :=
   {
     tot_fail_msg_fst_snd : msg_fail = tot_map_msg msg_fail
   }.
@@ -114,14 +119,13 @@ Section TotalMapBijective.
 Context `{MB : MultiParamsNameTotalMapBijective}.
 
 Lemma tot_map_name_injective : 
-forall n n', tot_map_name n = tot_map_name n' -> n = n'.
+  forall n n', tot_map_name n = tot_map_name n' -> n = n'.
 Proof.
 move => n n'.
 case (name_eq_dec n n') => H_dec //.
 move => H_eq.
-rewrite -(tot_map_name_inv_inverse n) in H_dec.
-rewrite H_eq in H_dec.
-by rewrite tot_map_name_inv_inverse in H_dec.
+case: H_dec.
+by rewrite -(tot_map_name_inv_inverse n) H_eq tot_map_name_inv_inverse.
 Qed.
 
 End TotalMapBijective.
@@ -134,9 +138,9 @@ Context {multi_fst : MultiParams base_fst}.
 Context {multi_snd : MultiParams base_snd}.
 Context {base_map : BaseParamsTotalMap base_fst base_snd}.
 Context {name_map : MultiParamsNameTotalMap multi_fst multi_snd}.
-Context {multi_map : MultiParamsTotalMap multi_fst multi_snd}.
+Context {msg_map : MultiParamsMsgTotalMap multi_fst multi_snd}.
 Context {name_map_bijective : MultiParamsNameTotalMapBijective name_map}.
-Context {multi_map_congr : MultiParamsTotalMapCongruency base_map name_map multi_map}.
+Context {multi_map_congr : MultiParamsTotalMapCongruency base_map name_map msg_map}.
 
 Definition tot_map_trace_occ (e : @name _ multi_fst * (@input base_fst + list (@output base_fst))) :=
 match e with
@@ -151,7 +155,8 @@ match p with
 end.
 
 Definition tot_map_net (net : @network _ multi_fst) : @network _ multi_snd :=
-mkNetwork (map tot_map_packet net.(nwPackets)) (fun n => tot_map_data (net.(nwState) (tot_map_name_inv n))).
+  {| nwPackets := map tot_map_packet net.(nwPackets) ;
+     nwState := fun n => tot_map_data (net.(nwState) (tot_map_name_inv n)) |}.
 
 Lemma tot_map_update_eq :
   forall f d h,
@@ -161,11 +166,9 @@ Proof.
 move => net d h.
 apply functional_extensionality => n.
 rewrite /update /=.
-case (name_eq_dec _ _) => H_dec; case (name_eq_dec _ _) => H_dec' //.
-  rewrite -H_dec in H_dec'.
-  by rewrite tot_map_name_inverse_inv in H_dec'.
-rewrite H_dec' in H_dec.
-by rewrite tot_map_name_inv_inverse in H_dec.
+repeat break_match => //.
+- by find_reverse_rewrite; find_rewrite_lem tot_map_name_inverse_inv.
+- by find_rewrite; find_rewrite_lem tot_map_name_inv_inverse.
 Qed.
 
 Corollary tot_map_update_packet_eq :
@@ -173,30 +176,18 @@ forall f p d,
   (fun n : name => tot_map_data (update f (pDst p) d (tot_map_name_inv n))) =
   (update (fun n : name => tot_map_data (f (tot_map_name_inv n))) (pDst (tot_map_packet p)) (tot_map_data d)).
 Proof.
-move => f. 
+move => f.
 case => src dst m d.
 exact: tot_map_update_eq.
 Qed.
 
-Lemma tot_map_packet_app_eq :
-  forall l p ms ms',
-    map tot_map_packet (map (fun m : name * msg => {| pSrc := pDst p; pDst := fst m; pBody := snd m |}) l ++ ms ++ ms') = 
-    map (fun m : name * msg => {| pSrc := pDst (tot_map_packet p); pDst := fst m; pBody := snd m |}) (tot_map_name_msgs l) ++ map tot_map_packet ms ++ map tot_map_packet ms'.
-Proof.
-move => l; case => src dst m ms ms'.
-rewrite 2!map_app.
-elim: l => //=.
-case => /= n m' l IH.
-by rewrite IH.
-Qed.
-
-Lemma tot_map_packet_eq :
-  forall l l' h,
-    map tot_map_packet (map (fun m : name * msg => {| pSrc := h; pDst := fst m; pBody := snd m |}) l ++ l') =
-    map (fun m : name * msg => {| pSrc := tot_map_name h; pDst := fst m; pBody := snd m |}) (tot_map_name_msgs l) ++ map tot_map_packet l'.
+Lemma tot_map_packet_map_eq :
+  forall l h,
+    map tot_map_packet (map (fun m : name * msg => {| pSrc := h; pDst := fst m; pBody := snd m |}) l) = 
+    map (fun m : name * msg => {| pSrc := tot_map_name h; pDst := fst m; pBody := snd m |}) (tot_map_name_msgs l).
 Proof.
 elim => //=.
-case => n m l IH l' h.
+case => /= n m' l IH h.
 by rewrite IH.
 Qed.
 
@@ -204,8 +195,7 @@ Lemma tot_init_handlers_fun_eq :
     init_handlers = fun n : name => tot_map_data (init_handlers (tot_map_name_inv n)).
 Proof.
 apply functional_extensionality => n.
-rewrite tot_init_handlers_eq.
-by rewrite tot_map_name_inverse_inv.
+by rewrite tot_init_handlers_eq tot_map_name_inverse_inv.
 Qed.
 
 Lemma tot_map_trace_occ_inv : 
@@ -243,9 +233,9 @@ move => out.
 case => //=.
 move => h0.
 move => inp' out' H_eq.
-inversion H_eq; subst.
-apply tot_map_name_injective in H2.
-rewrite H2.
+inversion H_eq.
+find_apply_lem_hyp tot_map_name_injective.
+repeat find_rewrite.
 by exists h; exists inp; exists out.
 Qed.
 
@@ -270,7 +260,9 @@ case => {net net' tr}.
     by rewrite tot_map_name_inv_inverse.
   * rewrite /= H_eq' /= /tot_map_net /=.
     rewrite -tot_map_update_packet_eq.
-    by rewrite tot_map_packet_app_eq.
+    rewrite 2!map_app.
+    destruct p.
+    by rewrite tot_map_packet_map_eq.
 - move => h net net' out inp d l H_hnd H_eq.
   apply (@SM_input _ _ _ _ _ _ _ (tot_map_data d) (tot_map_name_msgs l)).
     rewrite /=.
@@ -280,8 +272,7 @@ case => {net net' tr}.
     rewrite H_q.
     by rewrite tot_map_name_inv_inverse.
   rewrite /= H_eq /= /tot_map_net /=.
-  rewrite -tot_map_update_eq.
-  by rewrite tot_map_packet_eq.
+  by rewrite -tot_map_update_eq map_app tot_map_packet_map_eq.
 Qed.
 
 Corollary step_m_tot_mapped_simulation_star_1 :
@@ -293,16 +284,16 @@ move => net tr H_step.
 remember step_m_init as y in *.
 move: Heqy.
 induction H_step using refl_trans_1n_trace_n1_ind => H_init /=.
-  rewrite H_init.
-  rewrite /step_m_init /= /tot_map_net /=.
+  rewrite H_init /step_m_init /= /tot_map_net /=.
   rewrite tot_init_handlers_fun_eq.
   exact: RT1nTBase.
 concludes.
-rewrite H_init in H_step2 H_step1.
-apply step_m_tot_mapped_simulation_1 in H.
+repeat find_rewrite.
+find_apply_lem_hyp step_m_tot_mapped_simulation_1.
 rewrite map_app.
-have H_trans := refl_trans_1n_trace_trans IHH_step1.
-apply: H_trans.
+match goal with
+| H : step_m_star _ _ _ |- _ => apply: (refl_trans_1n_trace_trans H)
+end.
 rewrite (app_nil_end (map _ _)).
 apply: (@RT1nTStep _ _ _ _ (tot_map_net x'')) => //.
 exact: RT1nTBase.
@@ -313,153 +304,137 @@ Theorem step_m_tot_mapped_simulation_2 :
       @step_m _ multi_snd net net' out ->
       tot_map_net mnet = net ->
       map tot_map_trace_occ mout = out ->
-      exists mnet',
-        @step_m _ multi_fst mnet mnet' mout /\
-        tot_map_net mnet' = net'.
+      exists mnet', @step_m _ multi_fst mnet mnet' mout /\
+      tot_map_net mnet' = net'.
 Proof.
 move => net net' out mnet mout H_step H_eq H_eq'.
 invcs H_step.
-- case: p H4 H H0 => /= src dst m H4 H H0.
+- destruct p.
   rewrite /tot_map_net /=.
-  case: mnet H H0 => /= pks sts H_eq H_hnd.
-  have [pks1 [pks2 [H_eq_pks [H_eq_pks1 H_eq_pks2]]]] := map_eq_inv _ _ _ _ H_eq.
+  destruct mnet.
+  rewrite /=.
+  match goal with
+  | H : map tot_map_packet _ = _ |- _ => 
+    have [pks1 [pks2 [H_eq_pks [H_eq_pks1 H_eq_pks2]]]] := map_eq_inv _ _ _ _ H
+  end.
   case: pks2 H_eq_pks H_eq_pks2 => //= p pks2 H_eq_pks H_eq_pks2.
   rewrite H_eq_pks.
   inversion H_eq_pks2.
-  case H_hnd': (net_handlers (pDst p) (pSrc p) (pBody p) (sts (pDst p))) => [dout l'].
+  case H_hnd': (net_handlers (Net.pDst p) (Net.pSrc p) (Net.pBody p) (nwState (Net.pDst p))) => [dout l'].
   case: dout H_hnd' => out' d' H_hnd'.
   rewrite -H_eq_pks1.
-  exists {| nwPackets := send_packets (pDst p) l' ++ pks1 ++ pks2 ; nwState := update sts (pDst p) d' |}.
+  exists {| nwPackets := send_packets (Net.pDst p) l' ++ pks1 ++ pks2 ; nwState := update nwState (Net.pDst p) d' |}.
   split.
-  * have [n' [lo [H_eq_mout [H_eq_n H_eq_lo]]]] := tot_map_trace_occ_inv _ (eq_sym H4).
+  * match goal with
+    | H : _ = map tot_map_trace_occ _ |- _ => 
+      have [n' [lo [H_eq_mout [H_eq_n H_eq_lo]]]] := tot_map_trace_occ_inv _ (eq_sym H)
+    end.
     rewrite H_eq_mout.
-    have H_eq_dst: n' = pDst p.
-      rewrite -(tot_map_name_inv_inverse n').
-      rewrite H_eq_n.
-      case: p H_eq_pks H_eq_pks2 H0 H_hnd' => src' dst' m' H_eq_pks H_eq_pks2 H0 H_hnd'.
-      rewrite /=.
-      rewrite /= in H0.
-      inversion H0.
+    have H_eq_dst: n' = Net.pDst p.
+      rewrite -(tot_map_name_inv_inverse n') H_eq_n.
+      destruct p.
+      find_inversion.
       by rewrite tot_map_name_inv_inverse.
     rewrite H_eq_dst.
     apply (@SM_deliver _ _ _ _ _ pks1 pks2 _ d' l') => //=.
     suff H_suff: lo = out' by rewrite H_suff.
-    have H_eq_hnd := @tot_net_handlers_eq _ _ _ _ _ _ _ multi_map_congr (pDst p) (pSrc p) (pBody p) (sts (pDst p)).
+    have H_eq_hnd := @tot_net_handlers_eq _ _ _ _ _ _ _ multi_map_congr (Net.pDst p) (Net.pSrc p) (Net.pBody p) (nwState (Net.pDst p)).
     rewrite /tot_mapped_net_handlers /= in H_eq_hnd.
     repeat break_let.
     inversion H_hnd'.
-    rewrite H2 H3 H5 in H_eq_hnd.
-    rewrite -{1}H_eq_dst H_eq_n in H_eq_hnd.
-    rewrite -H_eq_dst in H_eq_hnd.
-    rewrite -(tot_map_name_inv_inverse n') H_eq_n in H_eq_hnd.
-    move {Heqp1 Heqp0 H_hnd'}.
-    have H_eq_src: tot_map_name (pSrc p) = src.
-      case: p H_eq_pks H_eq_pks2 H0 H_eq_dst H_eq_hnd => src' dst' m' H_eq_pks H_eq_pks2 H0 H_eq_dst H_eq_hnd.
-      rewrite /=.
-      rewrite /= in H0.
-      by inversion H0.
+    simpl in *.
+    have H_eq_src: tot_map_name (Net.pSrc p) = pSrc by destruct p; simpl in *; find_inversion.
     rewrite H_eq_src /= {H_eq_src} in H_eq_hnd.
-    have H_eq_body: tot_map_msg (pBody p) = m.
-      case: p H_eq_pks H_eq_pks2 H0 H_eq_dst H_eq_hnd => src' dst' m' H_eq_pks H_eq_pks2 H0 H_eq_dst H_eq_hnd.
-      rewrite /=.
-      rewrite /= in H0.
-      by inversion H0.
-    rewrite H_eq_body H_hnd in H_eq_hnd.
-    inversion H_eq_hnd.
-    rewrite -H_eq_lo in H6.
-    symmetry.
-    move: H6.
-    apply map_eq_inv_eq.
-    exact: tot_map_output_injective.
-  * rewrite /=.
-    rewrite /update /=.
-    have H_eq_dst: tot_map_name (pDst p) = dst.
-      case: p H_eq_pks H_eq_pks2 H0 H_hnd' => src' dst' m' H_eq_pks H_eq_pks2 H0 H_hnd'.
-      by inversion H0.
-    have H_eq_src: tot_map_name (pSrc p) = src.
-      case: p H_eq_pks H_eq_pks2 H0 H_hnd' H_eq_dst => src' dst' m' H_eq_pks H_eq_pks2 H0 H_hnd' H_eq_dst.
-      by inversion H0.
-    have H_eq_body: tot_map_msg (pBody p) = m.
-      case: p H_eq_pks H_eq_pks2 H0 H_eq_dst H_eq_src H_hnd' => src' dst' m' H_eq_pks H_eq_pks2 H0 H_eq_dst H_eq_src H_hnd'.
-      by inversion H0.
+    have H_eq_body: tot_map_msg (Net.pBody p) = pBody by destruct p; simpl in *; find_inversion.
+    rewrite H_eq_body in H_eq_hnd.
+    match goal with
+    | H: net_handlers _ _ _ (tot_map_data (_ (tot_map_name_inv pDst))) = _ |- _ => 
+      rewrite -H_eq_n tot_map_name_inv_inverse H_eq_dst in H ;
+        rewrite H in H_eq_hnd
+    end.
+    find_inversion.
+    find_apply_lem_hyp map_eq_inv_eq; last exact: tot_map_output_injective.
+    by symmetry.
+  * rewrite /= /update /=.
+    have H_eq_dst: tot_map_name (Net.pDst p) = pDst by destruct p; find_inversion.
+    have H_eq_src: tot_map_name (Net.pSrc p) = pSrc by destruct p; find_inversion.
+    have H_eq_body: tot_map_msg (Net.pBody p) = pBody by destruct p; find_inversion.
     rewrite 2!map_app.
-    have H_eq_hnd := @tot_net_handlers_eq _ _ _ _ _ _ _ multi_map_congr (pDst p) (pSrc p) (pBody p) (sts (pDst p)).
+    have H_eq_hnd := @tot_net_handlers_eq _ _ _ _ _ _ _ multi_map_congr (Net.pDst p) (Net.pSrc p) (Net.pBody p) (nwState (Net.pDst p)).
     rewrite /tot_mapped_net_handlers /= in H_eq_hnd.
     repeat break_let.
     inversion H_hnd'.
     rewrite H_eq_dst H_eq_src H_eq_body in H_eq_hnd.
-    rewrite -{2}H_eq_dst tot_map_name_inv_inverse in H_hnd.
-    rewrite H_hnd in H_eq_hnd.
-    inversion H_eq_hnd.
-    rewrite H2 in H6.
-    rewrite H3 in H7.
-    rewrite H5 in H8.
-    rewrite H3 H5.
+    simpl in *.       
+    match goal with
+    | H: net_handlers _ _ _ (tot_map_data (_ (tot_map_name_inv pDst))) = _ |- _ => 
+      rewrite -{2}H_eq_dst tot_map_name_inv_inverse in H;
+        rewrite H in H_eq_hnd
+    end.
+    find_inversion; clean.
     set nwP1 := map tot_map_packet _.
     set nwP2 := map (fun _ => _) (tot_map_name_msgs _).
     set nwS1 := fun _ => _.
     set nwS2 := fun _ => _.
     have H_eq_nw: nwP1 = nwP2.
-      rewrite /nwP1 /nwP2 {H_hnd' H5 H8 nwP1 nwP2}.
-      elim: l' => //=.
-      case => /= n' m' l' IH.
+      rewrite /nwP1 /nwP2.
+      elim l' => //=.
+      case => /= n' m' l0 IH.
       rewrite IH.
-      by rewrite H_eq_dst.
-    rewrite -H_eq_nw /nwP1 {H_eq_nw nwP1 nwP2}.
+      by find_rewrite.
+    rewrite -H_eq_nw /nwP1 {H_eq_nw nwP1 nwP2}.    
     have H_eq_sw: nwS1 = nwS2.
       rewrite /nwS1 /nwS2.
       apply functional_extensionality => n'.
-      rewrite -H_eq_dst.
-      case (name_eq_dec _ _) => H_dec.
-        rewrite -H_dec.
-        rewrite tot_map_name_inverse_inv.
-        by case (name_eq_dec _ _).
-      case (name_eq_dec _ _) => H_dec' //.
-      rewrite H_dec' in H_dec.
-      by rewrite tot_map_name_inv_inverse in H_dec.
+      repeat break_if => //.
+      + find_reverse_rewrite. 
+        by find_rewrite_lem tot_map_name_inverse_inv.
+      + find_rewrite. 
+        by find_rewrite_lem tot_map_name_inv_inverse.
     by rewrite H_eq_sw.
 - rewrite /tot_map_net /=.
-  case: mnet H => /= pks sts H_hnd.
-  have [h' [inp' [out' [H_eq_mout [H_eq_n [H_eq_out H_eq_inp]]]]]] := tot_map_trace_occ_in_inv _ (eq_sym H3).
-  have H_q := @tot_input_handlers_eq _ _ _ _ _ _ _ multi_map_congr h' inp' (sts h').
+  destruct mnet.
+  simpl in *.
+  match goal with
+  | H: _ = map tot_map_trace_occ _ |- _ => 
+    have [h' [inp' [out' [H_eq_mout [H_eq_n [H_eq_out H_eq_inp]]]]]] := tot_map_trace_occ_in_inv _ (eq_sym H)
+  end.
+  have H_q := @tot_input_handlers_eq _ _ _ _ _ _ _ multi_map_congr h' inp' (nwState h').
   rewrite /tot_mapped_input_handlers in H_q.
   repeat break_let.
   rewrite H_eq_n H_eq_inp in H_q.
-  rewrite -{2}H_eq_n tot_map_name_inv_inverse in H_hnd.
-  rewrite H_hnd in H_q.
-  inversion H_q.
-  rewrite -H_eq_out in H0.
-  rewrite H1 H2.
-  exists ({| nwPackets := send_packets h' l0 ++ pks ; nwState := update sts h' d0 |}).
+  match goal with
+    | H: input_handlers _ _ (tot_map_data (_ (tot_map_name_inv h))) = _ |- _ => 
+      rewrite -{2}H_eq_n tot_map_name_inv_inverse in H;
+        rewrite H in H_q
+  end.
+  find_inversion.
+  find_inversion.
+  exists ({| nwPackets := send_packets h' l0 ++ nwPackets ; nwState := update nwState h' d0 |}).
   split.
-  * rewrite H_eq_mout.
-    apply (@SM_input _ _ _ _ _ _ _ d0 l0) => //.
-    rewrite /= Heqp.
+  * apply (@SM_input _ _ _ _ _ _ _ d0 l0) => //=.
+    find_rewrite.
     suff H_suff: l1 = out' by rewrite H_suff.
-    move: H0.
-    apply map_eq_inv_eq.
-    exact: tot_map_output_injective.
+    by find_apply_lem_hyp map_eq_inv_eq; last exact: tot_map_output_injective.
   * rewrite /= map_app.
     set nwP1 := map tot_map_packet _.
-    set nwP2 := map (fun _ => _) l.
+    set nwP2 := map (fun _ => _) (tot_map_name_msgs _).
     set nwS1 := fun _ => _.
     set nwS2 := update _ _ _.
     have H_eq_nwp: nwP1 = nwP2.
-      rewrite /nwP1 /nwP2 {Heqp H_q nwP1 nwP2}.
-      rewrite -H2 {H2}.
-      elim: l0 => //=.
-      case => /= n m l0 IH.
-      by rewrite H_eq_n IH.
+      rewrite /nwP1 /nwP2 {nwP1 nwP2}.
+      elim l0 => //=.
+      case => /= n m l' IH.
+      by rewrite IH.
     have H_eq_nws: nwS1 = nwS2.
       rewrite /nwS1 /nwS2.
       rewrite /update /=.
       apply functional_extensionality => n.
-      rewrite -H_eq_n -H1.
-      case (name_eq_dec _ _) => H_dec.
-        case (name_eq_dec _ _) => H_dec' //.
-        by rewrite -H_dec tot_map_name_inverse_inv in H_dec'.
-      case (name_eq_dec _ _) => H_dec' //.
-      by rewrite H_dec' tot_map_name_inv_inverse in H_dec.
+      repeat break_if => //.
+      + find_reverse_rewrite. 
+        by find_rewrite_lem tot_map_name_inverse_inv.
+      + find_rewrite.
+        by find_rewrite_lem tot_map_name_inv_inverse.
     by rewrite H_eq_nwp H_eq_nws.
 Qed.
 
@@ -511,11 +486,9 @@ Proof.
 move => h.
 elim => //=.
 move => n failed IH.
-case (name_eq_dec _ _) => H_eq; case (name_eq_dec _ _) => H_eq' //.
-- by rewrite H_eq in H_eq'.
-- rewrite -(tot_map_name_inv_inverse h) in H_eq.
-  rewrite H_eq' in H_eq.
-  by rewrite tot_map_name_inv_inverse in H_eq.
+repeat break_if => //.
+- by find_rewrite.
+- by find_apply_lem_hyp tot_map_name_injective.
 - by rewrite /= IH.
 Qed.
 
@@ -535,12 +508,12 @@ forall h net,
 Proof.
 move => h net.
 apply: functional_extensionality => n.
-case (name_eq_dec _ _) => H_dec; case (name_eq_dec _ _) => H_dec' //.
+repeat break_if => //.
 - by rewrite tot_reboot_eq.
-- rewrite -H_dec in H_dec'.
-  by rewrite tot_map_name_inverse_inv in H_dec'.
-- rewrite H_dec' in H_dec.
-  by rewrite tot_map_name_inv_inverse in H_dec.
+- find_reverse_rewrite.
+  by find_rewrite_lem tot_map_name_inverse_inv.
+- find_rewrite.
+  by find_rewrite_lem tot_map_name_inv_inverse.
 Qed.
 
 Theorem step_f_tot_mapped_simulation_1 :
@@ -550,43 +523,48 @@ Theorem step_f_tot_mapped_simulation_1 :
 Proof.
 move => net net' failed failed' tr H_step.
 invcs H_step.
-- have ->: tot_map_name (pDst p) = pDst (tot_map_packet p) by case: p H3 H4 H6 => src dst m.
+- have ->: tot_map_name (pDst p) = pDst (tot_map_packet p) by destruct p.
   apply (@SF_deliver _ _ _ _ _ _ _ (map tot_map_packet xs) (map tot_map_packet ys) _ (tot_map_data d) (tot_map_name_msgs l)).
-  * by rewrite /tot_map_net /= H3 /= map_app.
-  * case: p H3 H4 H6 => /= src dst m H3 H4 H6.
+  * rewrite /tot_map_net /=.
+    find_rewrite.
+    by rewrite map_app.
+  * destruct p.
     exact: not_in_failed_not_in.
-  * case: p H3 H4 H6 => /= src dst m H3 H4 H6.        
-    have H_q := tot_net_handlers_eq dst src m (nwState net dst).
+  * destruct p.
+    simpl in *.
+    have H_q := tot_net_handlers_eq pDst pSrc pBody (nwState net pDst).
     rewrite /tot_mapped_net_handlers in H_q.
-    rewrite H6 in H_q.
+    find_rewrite.
     rewrite H_q.
     by rewrite tot_map_name_inv_inverse.
-  * rewrite /= -tot_map_update_packet_eq /=.
-    rewrite /tot_map_net /=.
-    by rewrite tot_map_packet_app_eq.
+  * rewrite /= -tot_map_update_packet_eq /= /tot_map_net /=.
+    destruct p.
+    by rewrite 2!map_app tot_map_packet_map_eq.
 - apply (@SF_input _ _ _ _ _ _ _ _ _ (tot_map_data d) (tot_map_name_msgs l)).
   * exact: not_in_failed_not_in.
   * rewrite /=.
     have H_q := tot_input_handlers_eq h inp (nwState net h).
     rewrite /tot_mapped_input_handlers /= in H_q.
-    rewrite H5 in H_q.
+    find_rewrite.
     rewrite H_q.
     by rewrite tot_map_name_inv_inverse.
-  * rewrite /= /tot_map_net /=.
-    rewrite -tot_map_update_eq.
-    by rewrite tot_map_packet_eq.
+  * rewrite /= /tot_map_net /= -tot_map_update_eq.
+    by rewrite map_app tot_map_packet_map_eq.
 - apply (@SF_drop _ _ _ _ _ _ (tot_map_packet p) (map tot_map_packet xs) (map tot_map_packet ys)).
-  * by rewrite /tot_map_net /= H4 map_app.
+  * rewrite /tot_map_net /=.
+    find_rewrite.
+    by rewrite map_app.
   * by rewrite /tot_map_net /= map_app.
 - apply (@SF_dup _ _ _ _ _ _ (tot_map_packet p) (map tot_map_packet xs) (map tot_map_packet ys)).
-  * by rewrite /tot_map_net /= H4 map_app.
+  * rewrite /tot_map_net /=.
+    find_rewrite.
+    by rewrite map_app.
   * by rewrite /tot_map_net /= map_app.
 - exact: SF_fail.
 - apply: (SF_reboot (tot_map_name h)).
   * exact: in_failed_in.
   * by rewrite remove_tot_map_eq.
-  * rewrite /tot_map_net /=.
-    by rewrite tot_map_reboot_eq.
+  * by rewrite /tot_map_net /= tot_map_reboot_eq.
 Qed.
 
 Corollary step_f_tot_mapped_simulation_star_1 :
@@ -596,28 +574,24 @@ Corollary step_f_tot_mapped_simulation_star_1 :
 Proof.
 move => net failed tr H_step.
 remember step_f_init as y in *.
-have H_eq_f: failed = fst (failed, net) by [].
-have H_eq_n: net = snd (failed, net) by [].
-rewrite H_eq_f {H_eq_f}.
-rewrite {2}H_eq_n {H_eq_n}.
+change failed with (fst (failed, net)).
+change net with (snd (failed, net)) at 2.
 move: Heqy.
 induction H_step using refl_trans_1n_trace_n1_ind => H_init /=.
-  rewrite H_init.
-  rewrite /step_f_init /= /step_m_init /tot_map_net /=.
-  rewrite tot_init_handlers_fun_eq.
+  rewrite H_init /step_f_init /= /step_m_init /tot_map_net /= tot_init_handlers_fun_eq.
   exact: RT1nTBase.
 concludes.
-rewrite H_init {H_init x} in H_step2 H_step1.
-case: x' H IHH_step1 H_step1 => failed' net'.
-case: x'' H_step2 => failed'' net''.
+repeat find_rewrite.
+destruct x'.
+destruct x''.
 rewrite /=.
-move => H_step2 H IHH_step1 H_step1.
-apply step_f_tot_mapped_simulation_1 in H.
+find_apply_lem_hyp step_f_tot_mapped_simulation_1.
 rewrite map_app.
-have H_trans := refl_trans_1n_trace_trans IHH_step1.
-apply: H_trans.
+match goal with
+| H : step_f_star _ _ _ |- _ => apply: (refl_trans_1n_trace_trans H)
+end.
 rewrite (app_nil_end (map tot_map_trace_occ _)).
-apply (@RT1nTStep _ _ _ _ (map tot_map_name failed'', tot_map_net net'')) => //.
+apply (@RT1nTStep _ _ _ _ (map tot_map_name l0, tot_map_net n0)) => //.
 exact: RT1nTBase.
 Qed.
 
@@ -630,8 +604,9 @@ move => n l IH.
 case => //=.
 move => n' l' H_eq.
 inversion H_eq.
-apply tot_map_name_injective in H0.
-by rewrite H0 (IH l').
+find_apply_lem_hyp tot_map_name_injective.
+find_eapply_lem_hyp IH.
+by repeat find_rewrite.
 Qed.
 
 Theorem step_f_tot_mapped_simulation_2 :
@@ -641,236 +616,241 @@ Theorem step_f_tot_mapped_simulation_2 :
       map tot_map_name mfailed = failed ->
       map tot_map_name mfailed' = failed' ->
       map tot_map_trace_occ mout = out ->
-      exists mnet',
-        @step_f _ _ fail_fst (mfailed, mnet) (mfailed', mnet') mout /\
-        tot_map_net mnet' = net'.
+      exists mnet', @step_f _ _ fail_fst (mfailed, mnet) (mfailed', mnet') mout /\
+      tot_map_net mnet' = net'.
 Proof.
 move => net net' failed failed' out mnet mfailed mfailed' mout H_step H_eq_net H_eq_f H_eq_f' H_eq_out.
 invcs H_step.
-- case: p H4 H5 H3 H6 => /= src dst m H4 H5 H3 H6.
+- destruct p.
   rewrite /tot_map_net /=.
-  case: mnet H3 H6 => /= pks sts H_eq H_hnd.
-  have [pks1 [pks2 [H_eq_pks [H_eq_pks1 H_eq_pks2]]]] := map_eq_inv _ _ _ _ H_eq.
+  destruct mnet.
+  simpl in *.
+  match goal with
+  | H : map tot_map_packet _ = _ |- _ => 
+    have [pks1 [pks2 [H_eq_pks [H_eq_pks1 H_eq_pks2]]]] := map_eq_inv _ _ _ _ H
+  end.
   case: pks2 H_eq_pks H_eq_pks2 => //= p pks2 H_eq_pks H_eq_pks2.
   rewrite H_eq_pks.
   inversion H_eq_pks2.
-  case H_hnd': (net_handlers (pDst p) (pSrc p) (pBody p) (sts (pDst p))) => [dout l'].
+  case H_hnd': (net_handlers (Net.pDst p) (Net.pSrc p) (Net.pBody p) (nwState (Net.pDst p))) => [dout l'].
   case: dout H_hnd' => out' d' H_hnd'.
   rewrite -H_eq_pks1.
-  exists {| nwPackets := send_packets (pDst p) l' ++ pks1 ++ pks2 ; nwState := update sts (pDst p) d' |}.
+  exists {| nwPackets := send_packets (Net.pDst p) l' ++ pks1 ++ pks2 ; nwState := update nwState (Net.pDst p) d' |}.
   split.
-  * have [n' [lo [H_eq_mout [H_eq_n H_eq_lo]]]] := tot_map_trace_occ_inv _ (eq_sym H5).
+  * match goal with
+    | H : _ = map tot_map_trace_occ _ |- _ => 
+      have [n' [lo [H_eq_mout [H_eq_n H_eq_lo]]]] := tot_map_trace_occ_inv _ (eq_sym H)
+    end.
     rewrite H_eq_mout.
-    have H_eq_dst: n' = pDst p.
-      rewrite -(tot_map_name_inv_inverse n').
-      rewrite H_eq_n.
-      case: p H_eq_pks H_eq_pks2 H0 H_hnd' => src' dst' m' H_eq_pks H_eq_pks2 H0 H_hnd'.
-      rewrite /=.
-      rewrite /= in H0.
-      inversion H0.
+    have H_eq_dst: n' = Net.pDst p.
+      rewrite -(tot_map_name_inv_inverse n') H_eq_n.
+      destruct p.
+      simpl in *.
+      find_inversion.
       by rewrite tot_map_name_inv_inverse.
     rewrite H_eq_dst.
-    apply map_eq_name_eq_eq in H1.
-    rewrite H1.    
+    match goal with
+    | H: map tot_map_name _ = map tot_map_name _ |- _ =>
+      apply map_eq_name_eq_eq in H; rewrite H
+    end.
     apply (@SF_deliver _ _ _ _ _ _ _ pks1 pks2 _ d' l') => //=.
-      rewrite -H_eq_dst.
-      rewrite -H_eq_n in H4.
-      move => H_in.
-      by apply in_failed_in in H_in.
+      rewrite -H_eq_dst => H_in.
+      find_apply_lem_hyp in_failed_in.
+      by find_rewrite_lem H_eq_n.
     suff H_suff: lo = out' by rewrite H_suff.
-    have H_eq_hnd := @tot_net_handlers_eq _ _ _ _ _ _ _ multi_map_congr (pDst p) (pSrc p) (pBody p) (sts (pDst p)).
+    have H_eq_hnd := @tot_net_handlers_eq _ _ _ _ _ _ _ multi_map_congr (Net.pDst p) (Net.pSrc p) (Net.pBody p) (nwState (Net.pDst p)).
     rewrite /tot_mapped_net_handlers /= in H_eq_hnd.
     repeat break_let.
     inversion H_hnd'.
-    rewrite H3 H6 H7 in H_eq_hnd.
-    rewrite -{1}H_eq_dst H_eq_n in H_eq_hnd.
-    rewrite -H_eq_dst in H_eq_hnd.
-    rewrite -(tot_map_name_inv_inverse n') H_eq_n in H_eq_hnd.
-    move {Heqp1 Heqp0 H_hnd'}.
-    have H_eq_src: tot_map_name (pSrc p) = src.
-      case: p H_eq_pks H_eq_pks2 H0 H_eq_dst H_eq_hnd => src' dst' m' H_eq_pks H_eq_pks2 H0 H_eq_dst H_eq_hnd.
-      rewrite /=.
-      rewrite /= in H0.
-      by inversion H0.
+    have H_eq_src: tot_map_name (Net.pSrc p) = pSrc by destruct p; simpl in *; find_inversion.
     rewrite H_eq_src /= {H_eq_src} in H_eq_hnd.
-    have H_eq_body: tot_map_msg (pBody p) = m.
-      case: p H_eq_pks H_eq_pks2 H0 H_eq_dst H_eq_hnd => src' dst' m' H_eq_pks H_eq_pks2 H0 H_eq_dst H_eq_hnd.
-      rewrite /=.
-      rewrite /= in H0.
-      by inversion H0.
-    rewrite H_eq_body H_hnd in H_eq_hnd.
-    inversion H_eq_hnd.
-    rewrite -H_eq_lo in H8.
-    symmetry.
-    move: H8.
-    apply map_eq_inv_eq.
-    exact: tot_map_output_injective.
-  * rewrite /=.
-    rewrite /update /=.
-    have H_eq_dst: tot_map_name (pDst p) = dst.
-      case: p H_eq_pks H_eq_pks2 H0 H_hnd' => src' dst' m' H_eq_pks H_eq_pks2 H0 H_hnd'.
-      by inversion H0.
-    have H_eq_src: tot_map_name (pSrc p) = src.
-      case: p H_eq_pks H_eq_pks2 H0 H_hnd' H_eq_dst => src' dst' m' H_eq_pks H_eq_pks2 H0 H_hnd' H_eq_dst.
-      by inversion H0.
-    have H_eq_body: tot_map_msg (pBody p) = m.
-      case: p H_eq_pks H_eq_pks2 H0 H_eq_dst H_eq_src H_hnd' => src' dst' m' H_eq_pks H_eq_pks2 H0 H_eq_dst H_eq_src H_hnd'.
-      by inversion H0.
+    have H_eq_body: tot_map_msg (Net.pBody p) = pBody by destruct p; simpl in *; find_inversion.
+    rewrite H_eq_body in H_eq_hnd.
+    match goal with
+    | H: net_handlers _ _ _ (tot_map_data (_ (tot_map_name_inv pDst))) = _ |- _ => 
+      rewrite -H_eq_n tot_map_name_inv_inverse H_eq_dst in H ;
+        rewrite H in H_eq_hnd
+    end.
+    find_inversion.
+    find_apply_lem_hyp map_eq_inv_eq; last exact: tot_map_output_injective.
+    by symmetry.
+  * rewrite /= /update /=.
+    have H_eq_dst: tot_map_name (Net.pDst p) = pDst by destruct p; simpl in *; find_inversion.
+    have H_eq_src: tot_map_name (Net.pSrc p) = pSrc by destruct p; simpl in *; find_inversion.
+    have H_eq_body: tot_map_msg (Net.pBody p) = pBody by destruct p; simpl in *; find_inversion.
     rewrite 2!map_app.
-    have H_eq_hnd := @tot_net_handlers_eq _ _ _ _ _ _ _ multi_map_congr (pDst p) (pSrc p) (pBody p) (sts (pDst p)).
+    have H_eq_hnd := @tot_net_handlers_eq _ _ _ _ _ _ _ multi_map_congr (Net.pDst p) (Net.pSrc p) (Net.pBody p) (nwState (Net.pDst p)).
     rewrite /tot_mapped_net_handlers /= in H_eq_hnd.
     repeat break_let.
     inversion H_hnd'.
     rewrite H_eq_dst H_eq_src H_eq_body in H_eq_hnd.
-    rewrite -{2}H_eq_dst tot_map_name_inv_inverse in H_hnd.
-    rewrite H_hnd in H_eq_hnd.
-    inversion H_eq_hnd.
-    rewrite H3 in H8.
-    rewrite H6 in H9.
-    rewrite H7 in H10.
-    rewrite H6 H7.
+    simpl in *.
+    match goal with
+    | H: net_handlers _ _ _ (tot_map_data (_ (tot_map_name_inv pDst))) = _ |- _ => 
+      rewrite -{2}H_eq_dst tot_map_name_inv_inverse in H;
+        rewrite H in H_eq_hnd
+    end.
+    find_inversion; clean.
     set nwP1 := map tot_map_packet _.
     set nwP2 := map (fun _ => _) (tot_map_name_msgs _).
     set nwS1 := fun _ => _.
     set nwS2 := fun _ => _.
     have H_eq_nw: nwP1 = nwP2.
-      rewrite /nwP1 /nwP2 {H_hnd' H7 H10 nwP1 nwP2}.
-      elim: l' => //=.
-      case => /= n' m' l' IH.
+      rewrite /nwP1 /nwP2.
+      elim l' => //=.
+      case => /= n' m' l0 IH.
       rewrite IH.
-      by rewrite H_eq_dst.
+      by find_rewrite.
     rewrite -H_eq_nw /nwP1 {H_eq_nw nwP1 nwP2}.
     have H_eq_sw: nwS1 = nwS2.
       rewrite /nwS1 /nwS2.
       apply functional_extensionality => n'.
-      rewrite -H_eq_dst.
-      case (name_eq_dec _ _) => H_dec.
-        rewrite -H_dec.
-        rewrite tot_map_name_inverse_inv.
-        by case (name_eq_dec _ _).
-      case (name_eq_dec _ _) => H_dec' //.
-      rewrite H_dec' in H_dec.
-      by rewrite tot_map_name_inv_inverse in H_dec.
+      repeat break_if => //.
+      + find_reverse_rewrite. 
+        by find_rewrite_lem tot_map_name_inverse_inv.
+      + find_rewrite. 
+        by find_rewrite_lem tot_map_name_inv_inverse.
     by rewrite H_eq_sw.
 - rewrite /tot_map_net /=.
-  case: mnet H5 => /= pks sts H_hnd.
-  have [h' [inp' [out' [H_eq_mout [H_eq_n [H_eq_out H_eq_inp]]]]]] := tot_map_trace_occ_in_inv _ (eq_sym H4).
-  have H_q := @tot_input_handlers_eq _ _ _ _ _ _ _ multi_map_congr h' inp' (sts h').
+  destruct mnet.
+  match goal with
+  | H: _ = map tot_map_trace_occ _ |- _ => 
+    have [h' [inp' [out' [H_eq_mout [H_eq_n [H_eq_out H_eq_inp]]]]]] := tot_map_trace_occ_in_inv _ (eq_sym H)
+  end.
+  have H_q := @tot_input_handlers_eq _ _ _ _ _ _ _ multi_map_congr h' inp' (nwState h').
   rewrite /tot_mapped_input_handlers in H_q.
   repeat break_let.
   rewrite H_eq_n H_eq_inp in H_q.
-  rewrite -{2}H_eq_n tot_map_name_inv_inverse in H_hnd.
-  rewrite H_hnd in H_q.
+  match goal with
+    | H: input_handlers _ _ (tot_map_data (_ (tot_map_name_inv h))) = _ |- _ => 
+      rewrite -{2}H_eq_n tot_map_name_inv_inverse in H ;
+        rewrite H in H_q
+    end.
   inversion H_q.
-  rewrite -H_eq_out in H0.
-  rewrite H2 H5.
-  apply map_eq_name_eq_eq in H1.
-  rewrite -H1.
-  rewrite -H1 in H3.
-  exists ({| nwPackets := send_packets h' l0 ++ pks ; nwState := update sts h' d0 |}).
+  simpl in *.
+  find_apply_lem_hyp map_eq_name_eq_eq.   
+  exists ({| nwPackets := send_packets h' l0 ++ nwPackets ; nwState := update nwState h' d0 |}).
   split.
   * rewrite H_eq_mout.
+    match goal with
+    | H: mfailed = _ |- _ => rewrite H
+    end.
     apply (@SF_input _ _ _ _ _ _ _ _ _ d0 l0) => //.      
-      rewrite -H_eq_n in H3.
       move => H_in.
-      by apply in_failed_in in H_in.
+      apply in_failed_in in H_in.
+      by rewrite H_eq_n in H_in.
     rewrite /= Heqp.
     suff H_suff: l1 = out' by rewrite H_suff.
-    move: H0.
-    apply map_eq_inv_eq.
-    exact: tot_map_output_injective.
+    match goal with
+    | H: map tot_map_output _ = _ |- _ => rewrite -H_eq_out in H
+    end.    
+    by find_apply_lem_hyp map_eq_inv_eq; last exact: tot_map_output_injective.
   * rewrite /= map_app.
     set nwP1 := map tot_map_packet _.
-    set nwP2 := map (fun _ => _) l.
+    set nwP2 := map (fun _ => _) (tot_map_name_msgs _).
     set nwS1 := fun _ => _.
     set nwS2 := update _ _ _.
     have H_eq_nwp: nwP1 = nwP2.
       rewrite /nwP1 /nwP2 {Heqp H_q nwP1 nwP2}.
-      rewrite -H5 {H5}.
-      elim: l0 => //=.
-      case => /= n m l0 IH.
+      elim l0 => //=.
+      case => /= n m l' IH.
       by rewrite H_eq_n IH.
     have H_eq_nws: nwS1 = nwS2.
       rewrite /nwS1 /nwS2.
       rewrite /update /=.
       apply functional_extensionality => n.
-      rewrite -H_eq_n -H2.
-      case (name_eq_dec _ _) => H_dec.
-        case (name_eq_dec _ _) => H_dec' //.
-        by rewrite -H_dec tot_map_name_inverse_inv in H_dec'.
-      case (name_eq_dec _ _) => H_dec' //.
-      by rewrite H_dec' tot_map_name_inv_inverse in H_dec.
+      rewrite -H_eq_n.
+      repeat break_if => //.
+      + match goal with
+        | H: _ = h' , H': _ <> tot_map_name h' |- _ => 
+          rewrite -H in H'
+        end.
+        by find_rewrite_lem tot_map_name_inverse_inv.
+      + match goal with
+        | H: n = _ , H': tot_map_name_inv n <> _ |- _ => 
+          rewrite H in H'
+        end.
+        by find_rewrite_lem tot_map_name_inv_inverse.
     by rewrite H_eq_nwp H_eq_nws.
-- case: mout H2 => // H_eq_mout {H_eq_mout}.
-  apply map_eq_name_eq_eq in H1.
-  rewrite -H1.
-  have [pks1 [pks2 [H_eq_pks [H_eq_pks1 H_eq_pks2]]]] := map_eq_inv _ _ _ _ H4.
+- destruct mout => //.
+  find_apply_lem_hyp map_eq_name_eq_eq.
+  find_reverse_rewrite.
+  match goal with
+  | H : map tot_map_packet _ = _ |- _ => 
+    have [pks1 [pks2 [H_eq_pks [H_eq_pks1 H_eq_pks2]]]] := map_eq_inv _ _ _ _ H
+  end.
   case: pks2 H_eq_pks H_eq_pks2 => //= p' pks2 H_eq_pks H_eq_pks2.
   inversion H_eq_pks2.
   rewrite -H_eq_pks1.
   exists {| nwPackets := pks1 ++ pks2 ; nwState := nwState mnet |}.
   split; first exact: (@SF_drop _ _ _ _ _ _ p' pks1 pks2).
   by rewrite /tot_map_net /= map_app.
-- case: mout H2 => // H_eq_mout {H_eq_mout}.
-  apply map_eq_name_eq_eq in H1.
-  rewrite -H1.
-  have [pks1 [pks2 [H_eq_pks [H_eq_pks1 H_eq_pks2]]]] := map_eq_inv _ _ _ _ H4.
+- destruct mout => //.
+  find_apply_lem_hyp map_eq_name_eq_eq.
+  find_rewrite.
+  match goal with
+  | H : map tot_map_packet _ = _ |- _ => 
+    have [pks1 [pks2 [H_eq_pks [H_eq_pks1 H_eq_pks2]]]] := map_eq_inv _ _ _ _ H
+  end.
   case: pks2 H_eq_pks H_eq_pks2 => //= p' pks2 H_eq_pks H_eq_pks2.
   inversion H_eq_pks2.
   rewrite -H_eq_pks1.
   exists {| nwPackets := p' :: pks1 ++ p' :: pks2 ; nwState := nwState mnet |}.
   split; first exact: (@SF_dup _ _ _ _ _ _ p' pks1 pks2).
-  by rewrite /tot_map_net /= map_app.
-- case: mout H2 => // H_eq_mout {H_eq_mout}.
-  case: mfailed' H => //= h' mfailed' H_eq.
-  inversion H_eq.
-  apply map_eq_name_eq_eq in H1.
-  rewrite -H1.
-  exists mnet.
+  by rewrite /tot_map_net /= map_app.  
+- destruct mout => //.
+  destruct mfailed' => //.
+  simpl in *.
+  find_inversion.
+  find_apply_lem_hyp map_eq_name_eq_eq.
+  find_rewrite.
+  exists mnet => //.
   split => //.
   exact: SF_fail.
-- case: mout H4 => // H_eq_mout {H_eq_mout}.
-  have H_in := H3.
-  apply in_split in H_in.
-  move: H_in => [ns1 [ns2 H_eq]].
-  have [mns1 [mns2 [H_eq_mns [H_eq_mns1 H_eq_mns2]]]] := map_eq_inv _ _ _ _ H_eq.
-  case: mns2 H_eq_mns H_eq_mns2 => //= h' mns2 H_eq_mns H_eq_mns2.
+- destruct mout => //.
+  find_copy_apply_lem_hyp in_split.
+  break_exists.
+  match goal with
+  | H: map tot_map_name _ = _ |- _ =>
+    have [mns1 [mns2 [H_eq_mns [H_eq_mns1 H_eq_mns2]]]] := map_eq_inv _ _ _ _ H
+  end.
+  destruct mns2 => //.
   exists {| nwPackets := nwPackets mnet ; 
-       nwState := (fun nm => match name_eq_dec nm h' with
+       nwState := (fun nm => match name_eq_dec nm n with
                            | left _ => (reboot (nwState mnet nm)) 
                            | right _ => (nwState mnet nm) 
                            end) |}.
   split.
-  * apply (@SF_reboot _ _ _ h') => //.
+  * apply (@SF_reboot _ _ _ n) => //.
     + rewrite H_eq_mns.
       apply in_or_app.
       by right; left.
     + inversion H_eq_mns2.
-      rewrite -H0 in H5.
-      move {H3 ns1 ns2 H_eq mns1 H_eq_mns1 h mns2 H_eq_mns H_eq_mns2 H0 H1}.
-      have H_eq: remove name_eq_dec (tot_map_name h') (map tot_map_name mfailed) = map tot_map_name (remove name_eq_dec h' mfailed).
-        move {H5 mfailed'}.
-        elim: mfailed => //=.
-        move => n l IH.
-        case (name_eq_dec _ _) => H_dec; case (name_eq_dec _ _) => H_dec' => //.
-        + by apply tot_map_name_injective in H_dec.
-        + by rewrite H_dec' in H_dec.
-        + by rewrite /= IH.               
-      rewrite H_eq in H5.
-      by apply map_eq_name_eq_eq in H5.
+      have H_eq: remove name_eq_dec h (map tot_map_name mfailed) = map tot_map_name (remove name_eq_dec n mfailed).
+        elim mfailed => //=.
+        move => n' l IH.
+        repeat break_if => //.
+        + by find_reverse_rewrite; find_apply_lem_hyp tot_map_name_injective.
+        + by find_reverse_rewrite; find_reverse_rewrite.
+        + by rewrite /= IH.
+      match goal with
+      | H: _ = remove _ _ _ |- _ => rewrite H_eq in H
+      end.
+      by find_apply_lem_hyp map_eq_name_eq_eq.
   * rewrite /tot_map_net /=.
     inversion H_eq_mns2.
     set nwS1 := fun _ => _.
     set nwS2 := fun _ => _.
     have H_eq_sw: nwS1 = nwS2.
       rewrite /nwS1 /nwS2 {nwS1 nwS2}.
-      apply functional_extensionality => n.
-      case (name_eq_dec _ _) => H_dec; case (name_eq_dec _ _) => H_dec' => //.
+      apply functional_extensionality => n'.
+      repeat break_if => //.
       + by rewrite tot_reboot_eq.
-      + rewrite -H_dec in H_dec'.
-        by rewrite tot_map_name_inverse_inv in H_dec'.
-      + rewrite H_dec' in H_dec.
-        by rewrite tot_map_name_inv_inverse in H_dec.
+      + by find_reverse_rewrite; find_rewrite_lem tot_map_name_inverse_inv.
+      + match goal with
+        | H: n' = _ , H': tot_map_name_inv n' <> _ |- _ => rewrite H in H'
+        end.
+        by find_rewrite_lem tot_map_name_inv_inverse.
     by rewrite H_eq_sw.
 Qed.
 
@@ -881,7 +861,7 @@ Proof.
 elim => /=; first by move => H_nd; exact: NoDup_nil.
 move => n ns IH H_nd.
 inversion H_nd.
-apply IH in H2.
+find_apply_lem_hyp IH.
 by apply NoDup_cons; first exact: not_in_failed_not_in.  
 Qed.
 
@@ -961,9 +941,9 @@ Qed.
 
 Lemma msg_in_map :
   forall m l n m',
-(forall nm, In nm l -> snd nm = m) ->
-In (tot_map_name n, tot_map_msg m') (map (fun nm : name * msg => (tot_map_name (fst nm), tot_map_msg (snd nm))) l) ->
-tot_map_msg m' = tot_map_msg m.
+    (forall nm, In nm l -> snd nm = m) ->
+    In (tot_map_name n, tot_map_msg m') (map (fun nm : name * msg => (tot_map_name (fst nm), tot_map_msg (snd nm))) l) ->
+    tot_map_msg m' = tot_map_msg m.
 Proof.
 move => m.
 elim => //=.
@@ -1018,9 +998,9 @@ Qed.
 
 Lemma in_tot_map_name :
 forall m l n,
-(forall nm, In nm l -> snd nm = m) ->
-In (n, tot_map_msg m) (map (fun nm : name * msg => (tot_map_name (fst nm), tot_map_msg (snd nm))) l) ->
-In (tot_map_name_inv n, m) l.
+  (forall nm, In nm l -> snd nm = m) ->
+  In (n, tot_map_msg m) (map (fun nm : name * msg => (tot_map_name (fst nm), tot_map_msg (snd nm))) l) ->
+  In (tot_map_name_inv n, m) l.
 Proof.
 move => m.
 elim => //=.
@@ -1039,9 +1019,9 @@ by right.
 Qed.
 
 Lemma in_msg_for_adjacent_to :
-forall m ns failed h n,
-In (tot_map_name_inv n, m) (msg_for m (adjacent_to_node h (exclude failed ns))) ->
-In (tot_map_name_inv n) (adjacent_to_node h (exclude failed ns)).
+  forall m ns failed h n,
+    In (tot_map_name_inv n, m) (msg_for m (adjacent_to_node h (exclude failed ns))) ->
+    In (tot_map_name_inv n) (adjacent_to_node h (exclude failed ns)).
 Proof.
 move => m.
 elim => //=.
@@ -1060,8 +1040,8 @@ Qed.
 
 Lemma in_adjacent_exclude_in_exlude :
   forall ns failed n h,
-In (tot_map_name_inv n) (adjacent_to_node h (exclude failed ns)) ->
-In (tot_map_name_inv n) (exclude failed ns) /\ adjacent_to h (tot_map_name_inv n).
+    In (tot_map_name_inv n) (adjacent_to_node h (exclude failed ns)) ->
+    In (tot_map_name_inv n) (exclude failed ns) /\ adjacent_to h (tot_map_name_inv n).
 Proof.
 elim => //=.
 move => n l IH failed n' h.
@@ -1087,8 +1067,8 @@ Qed.
 
 Lemma in_failed_exclude :
   forall ns failed n,
-  In (tot_map_name_inv n) (exclude failed ns) ->
-  ~ In (tot_map_name_inv n) failed /\ In (tot_map_name_inv n) ns.
+    In (tot_map_name_inv n) (exclude failed ns) ->
+    ~ In (tot_map_name_inv n) failed /\ In (tot_map_name_inv n) ns.
 Proof.
 elim => //=.
 move => n ns IH failed n'.
@@ -1110,7 +1090,7 @@ by right.
 Qed.
 
 Lemma in_in_adj_msg_for :
-      forall m ns failed n h,
+  forall m ns failed n h,
     In n ns ->
     ~ In n (map tot_map_name failed) ->
     adjacent_to h n ->
@@ -1166,7 +1146,7 @@ by right.
 Qed.
 
 Lemma not_in_map_not_in_failed :
-    forall failed n,
+  forall failed n,
     ~ In n (map tot_map_name failed) ->
     ~ In (tot_map_name_inv n) failed.
 Proof.
@@ -1185,9 +1165,9 @@ Qed.
 
 Lemma in_tot_map_msg :
   forall m l n,
-(forall nm, In nm l -> snd nm = m) ->
-In (tot_map_name_inv n, m) l ->
-In (n, tot_map_msg m) (map (fun nm : name * msg => (tot_map_name (fst nm), tot_map_msg (snd nm))) l).
+    (forall nm, In nm l -> snd nm = m) ->
+    In (tot_map_name_inv n, m) l ->
+    In (n, tot_map_msg m) (map (fun nm : name * msg => (tot_map_name (fst nm), tot_map_msg (snd nm))) l).
 Proof.
 move => m.
 elim => //=.
@@ -1294,11 +1274,11 @@ Qed.
 
 Context {fail_msg_fst : FailMsgParams multi_fst}.
 Context {fail_msg_snd : FailMsgParams multi_snd}.
-Context {fail_msg_map_congr : FailMsgParamsTotalMapCongruency fail_msg_fst fail_msg_snd multi_map}.
+Context {fail_msg_map_congr : FailMsgParamsTotalMapCongruency fail_msg_fst fail_msg_snd msg_map}.
 
 Lemma map_msg_fail_eq :
   forall h failed,
-  Permutation 
+   Permutation 
     (map (fun nm : name * msg => (tot_map_name (fst nm), tot_map_msg (snd nm))) (msg_for msg_fail (adjacent_to_node h (exclude failed nodes)))) 
     (msg_for msg_fail (adjacent_to_node (tot_map_name h) (exclude (map tot_map_name failed) nodes))).
 Proof.
@@ -1308,8 +1288,8 @@ exact: map_msg_for_eq.
 Qed.
 
 Definition tot_map_onet (onet : @ordered_network _ multi_fst) : @ordered_network _ multi_snd :=
-mkONetwork (fun src dst => map tot_map_msg (onet.(onwPackets) (tot_map_name_inv src) (tot_map_name_inv dst)))
-           (fun n => tot_map_data (onet.(onwState) (tot_map_name_inv n))).
+  {| onwPackets := fun src dst => map tot_map_msg (onet.(onwPackets) (tot_map_name_inv src) (tot_map_name_inv dst)) ;
+     onwState := fun n => tot_map_data (onet.(onwState) (tot_map_name_inv n)) |}.
 
 Lemma map_msg_update2 : 
   forall f ms to from,
