core/PartialExtendedMapSimulations.v
@@ -76,14 +76,16 @@ Class MultiParamsPartialExtendedMapCongruency
       pt_ext_map_data (init_handlers n) n = init_handlers (tot_map_name n) ;
     pt_ext_net_handlers_some : forall me src m st m',
       pt_ext_map_msg m = Some m' ->
-      pt_ext_mapped_net_handlers me src m st = net_handlers (tot_map_name me) (tot_map_name src) m' (pt_ext_map_data st me) ;
+      pt_ext_mapped_net_handlers me src m st = 
+        net_handlers (tot_map_name me) (tot_map_name src) m' (pt_ext_map_data st me) ;
     pt_ext_net_handlers_none : forall me src m st out st' ps,
       pt_ext_map_msg m = None ->
       net_handlers me src m st = (out, st', ps) ->
       pt_ext_map_data st' me = pt_ext_map_data st me /\ pt_ext_map_name_msgs ps = [] ;
     pt_ext_input_handlers_some : forall me inp st inp',
       pt_ext_map_input inp me st = Some inp' ->
-      pt_ext_mapped_input_handlers me inp st = input_handlers (tot_map_name me) inp' (pt_ext_map_data st me) ;
+      pt_ext_mapped_input_handlers me inp st = 
+        input_handlers (tot_map_name me) inp' (pt_ext_map_data st me) ;
     pt_ext_input_handlers_none : forall me inp st out st' ps,
       pt_ext_map_input inp me st = None ->
       input_handlers me inp st = (out, st', ps) ->
@@ -111,7 +113,7 @@ Context {name_map_bijective : MultiParamsNameTotalMapBijective name_map}.
 Context {multi_map_congr : MultiParamsPartialExtendedMapCongruency name_map multi_map}.
 
 Lemma pt_ext_init_handlers_fun_eq : 
-    init_handlers = fun n : name => pt_ext_map_data (init_handlers (tot_map_name_inv n)) (tot_map_name_inv n).
+  init_handlers = fun n : name => pt_ext_map_data (init_handlers (tot_map_name_inv n)) (tot_map_name_inv n).
 Proof.
 apply functional_extensionality => n.
 have H_eq := pt_ext_init_handlers_eq.
@@ -146,7 +148,8 @@ by case pt_ext_map_packet.
 Qed.
 
 Definition pt_ext_map_net (net : @network  _ multi_fst) : @network _ multi_snd :=
-mkNetwork (pt_ext_map_packets net.(nwPackets)) (fun n => pt_ext_map_data (net.(nwState) (tot_map_name_inv n)) (tot_map_name_inv n)).
+  {| nwPackets := pt_ext_map_packets net.(nwPackets) ;
+     nwState := fun n => pt_ext_map_data (net.(nwState) (tot_map_name_inv n)) (tot_map_name_inv n) |}.
 
 Lemma pt_ext_map_name_msgs_app_distr : 
   forall l l',
@@ -158,30 +161,29 @@ rewrite /= IH.
 by case (pt_ext_map_msg _) => [m'|].
 Qed.
 
-Lemma pt_ext_map_packet_map_app_eq :
-  forall l h ms,
-    pt_ext_map_packets (map (fun m : name * msg => {| pSrc := h; pDst := fst m; pBody := snd m |}) l ++ ms) = 
-    map (fun m : name * msg => {| pSrc := tot_map_name h; pDst := fst m; pBody := snd m |}) (pt_ext_map_name_msgs l) ++ pt_ext_map_packets ms.
+Lemma pt_ext_map_packet_map_eq :
+  forall l h,
+    pt_ext_map_packets (map (fun m : name * msg => {| pSrc := h; pDst := fst m; pBody := snd m |}) l) = 
+    map (fun m : name * msg => {| pSrc := tot_map_name h; pDst := fst m; pBody := snd m |}) (pt_ext_map_name_msgs l).
 Proof.
-move => l h ms.
+move => l h.
 elim: l => //=.
 case => n m l IH.
 case (pt_ext_map_msg _) => [m'|] //.
 by rewrite IH.
 Qed.
 
-Lemma pt_ext_map_packet_app_eq :
-  forall l p p' ms ms',
+Lemma pt_ext_map_packet_eq_some :
+  forall l p p',
     pt_ext_map_packet p = Some p' ->
-    pt_ext_map_packets (map (fun m : name * msg => {| pSrc := pDst p; pDst := fst m; pBody := snd m |}) l ++ ms ++ ms') = 
-    map (fun m : name * msg => {| pSrc := pDst p'; pDst := fst m; pBody := snd m |}) (pt_ext_map_name_msgs l) ++ pt_ext_map_packets ms ++ pt_ext_map_packets ms'.
+    pt_ext_map_packets (map (fun m : name * msg => {| pSrc := pDst p; pDst := fst m; pBody := snd m |}) l) = 
+    map (fun m : name * msg => {| pSrc := pDst p'; pDst := fst m; pBody := snd m |}) (pt_ext_map_name_msgs l).
 Proof.
-move => l; case => /= src dst m p ms ms'.
+move => l; case => /= src dst m p.
 case H_m: (pt_ext_map_msg m) => [m'|] // H_eq.
 injection H_eq => H_eq_p.
 rewrite -H_eq_p /=.
-rewrite -pt_ext_map_packets_app_distr.
-exact: pt_ext_map_packet_map_app_eq.
+exact: pt_ext_map_packet_map_eq.
 Qed.
 
 Lemma pt_ext_map_update_eq :
@@ -263,8 +265,8 @@ case => {net net' tr}.
       rewrite H_hnd in H_q.
       rewrite H_q.
       by rewrite tot_map_name_inv_inverse.
-    * rewrite /= /pt_ext_map_net /=.
-      rewrite (pt_ext_map_packet_app_eq _ _ _ _ H_m).
+    * rewrite /= /pt_ext_map_net /= 2!pt_ext_map_packets_app_distr.
+      rewrite (pt_ext_map_packet_eq_some _ _ H_m).
       by rewrite (pt_ext_map_update_eq_some _ _ _ H_m).
   right.
   rewrite H_eq' /= {H_eq'}.
@@ -295,8 +297,7 @@ case => {net net' tr}.
       rewrite H_hnd in H_q.
       rewrite H_q.
       by rewrite tot_map_name_inv_inverse.
-    rewrite /= H_eq /= /pt_ext_map_net /=.  
-    rewrite pt_ext_map_packet_map_app_eq.
+    rewrite /= H_eq /= /pt_ext_map_net /= pt_ext_map_packets_app_distr pt_ext_map_packet_map_eq.
     by rewrite -pt_ext_map_update_eq.
   right.
   rewrite H_eq /pt_ext_map_net /=.
