systems/TreeStatic.v
@@ -553,7 +553,7 @@ Instance Tree_FailureRecorder_name_tot_map_bijective : MultiParamsNameTotalMapBi
     tot_map_name_inverse_inv := fun _ => Logic.eq_refl
   }.
 
-Instance Tree_FailureRecorder_multi_params_pt_map : MultiParamsPartialMap Tree_MultiParams FR.FailureRecorder_MultiParams :=
+Instance Tree_FailureRecorder_multi_params_pt_map : MultiParamsMsgPartialMap Tree_MultiParams FR.FailureRecorder_MultiParams :=
   {
     pt_map_msg := fun m => match m with Fail => Some FR.Fail | _ => None end ;
   }.
@@ -631,7 +631,7 @@ Instance Tree_FailureRecorder_name_overlay_params_tot_map_congruency : NameOverl
   }.
 
 Theorem Tree_Failed_pt_mapped_simulation_star_1 :
-forall net failed tr,
+  forall net failed tr,
     @step_o_f_star _ _ _ Tree_FailMsgParams step_o_f_init (failed, net) tr ->
     exists tr', @step_o_f_star _ _ _ FR.FailureRecorder_FailMsgParams step_o_f_init (failed, pt_map_onet net) tr' /\
     pt_trace_remove_empty_out (pt_map_trace tr) = pt_trace_remove_empty_out tr'.
